Fin_Sequence_TM (verified)

TM/Code/FinTM.v
@@ -4,26 +4,125 @@ Require Import TM.Combinators.SequentialComposition TM.Combinators.Match.
 
 Open Scope vector_scope.
 
-Lemma fin_to_nat_proj1_S (n : nat) (x : Fin.t n) :
-  S (proj1_sig (Fin.to_nat x)) = proj1_sig (Fin.to_nat (Fin.FS x)).
-Proof.
-  induction x.
-  - cbn. reflexivity.
-  - rewrite <- IHx. cbn. destruct (Fin.to_nat x). cbn. reflexivity.
-Qed.
+(* Compute the [n]th (encoded as a [nat] on tape 1) value of a sequence [it f n x] and
+ * terminate in state [inr (it f n x)]. *)
+Section Fin_Seq_TM.
 
-Lemma fin_encode_S (m : nat) (x : Fin.t m) :
-  (@encode _ (I_Fin (S m)) (Fin.FS x) = true :: @encode _ (I_Fin m) x).
-Proof.
-  unfold encode. cbn. unfold encode_list. cbn.
-  induction x.
-  - cbn in *. reflexivity.
-  - cbn in *. unfold encode_unit. cbn. unfold fin_to_nat.
-    replace (proj1_sig (Fin.to_nat (Fin.FS (Fin.FS x)))) with
-        (S (proj1_sig (Fin.to_nat (Fin.FS x)))).
-    cbn. auto. now apply fin_to_nat_proj1_S.
-Qed.
+  Variable X : finType.
+  Variable start : X.
+  Variable f : X -> X.
+  
+  Lemma it_S (n : nat) (x : X) :
+    it f n (f x) = f (it f n x).
+  Proof. induction n; cbn; congruence. Qed.
 
+  (* (inl start) is the initial state,
+   * (inl _) are the internal states,
+   * (inr _) are the final states, that stand for the corresponding decoding. *)
+  Definition fin_seq_states := FinType (EqType (X + X))%type.
+
+  Definition fin_seq_TM_trans_mono :
+    fin_seq_states -> option bool_fin -> fin_seq_states * (option bool_fin * move).
+  Proof.
+    intros q. destruct q as [x | y] eqn:E.
+    - (* inl x *)
+      intros [ [ | ] | ].
+      + (* Some true *)
+        apply (inl (f x), (None, R)). (* continue *)
+      + (* Some false *)
+        apply (inr x, (None, R)). (* terminate *)
+      + (* None *)
+       apply (inl x, (None, N)). (* unexpected end of tape -> diverge *)
+    - (* inr y *)
+      intros _. apply (inr y, (None, N)). (* terminal state *)
+  Defined.
+
+  Definition fin_seq_fin : fin_seq_states -> bool.
+  Proof.
+    destruct 1 as [ _ | _ ]; [apply false | apply true].
+  Defined.
+  
+  Definition Fin_Seq_TM : mTM bool_fin 0.
+  Proof.
+    apply Mk_Mono_TM with (states := fin_seq_states).
+    - apply fin_seq_TM_trans_mono.
+    - apply (inl start).
+    - apply fin_seq_fin.
+  Defined.
+
+  Definition Fin_Seq : { M : mTM bool_fin 0 & states M -> option X }.
+  Proof.
+    exists Fin_Seq_TM. intros [ _ | x ]; [apply None | apply (Some x)].
+  Defined.
+
+  Lemma Fin_Seq_terminates_in_Strong :
+    forall (tape1 : tape bool_fin) (rest : list bool_fin) (i : nat)
+      (x : X),
+      tape_local tape1 = encode i ++ rest ->
+      exists tape2, tape_local tape2 = rest /\
+               loopM (M := Fin_Seq_TM) (S i) (mk_mconfig (inl x) [|tape1|]) =
+               Some (mk_mconfig (inr (it f i x)) [|tape2|]).
+  Proof.
+    intros tape1 rest i. revert tape1 rest. induction i; intros; cbn in *.
+    - unfold step at 1. cbn.
+      replace (current tape1) with (Some false); [ | erewrite tape_local_current_cons; now eauto]. cbn.
+      unfold step at 1. cbn.
+      replace (current tape1) with (Some false); [ | erewrite tape_local_current_cons; now eauto]. cbn.
+      exists (tape_move_right tape1). split; auto. erewrite tape_local_move_right; eauto.
+    - assert (current tape1 = Some true) as H' by (erewrite tape_local_current_cons; eauto).
+      assert (tape_local (tape_move_right tape1) = encode_list encode_unit (repeat tt i) ++ rest)
+        as H'' by (erewrite tape_local_move_right; eauto).
+      unfold step at 1. cbn. rewrite !H'.
+      unfold it. cbn.
+      unfold step at 2. unfold step at 2. cbn. rewrite !H'. cbn.
+      unfold step at 2. cbn. rewrite !H'. cbn.
+
+      (* current (tape_move_right tape1) must not be None *)
+      destruct (current (tape_move_right tape1)) eqn:E1.
+      + destruct e eqn:E2; cbn in *.
+        * edestruct (IHi (tape_move_right tape1) rest (f x)) as (tape2&IHi'&IHi'').
+          eapply H''. cbn in *.
+          unfold step at 2. cbn. rewrite H'. cbn.
+          unfold step at 2 in IHi''. cbn in IHi''. rewrite E1 in IHi''. cbn in IHi''.
+          eexists tape2. split; auto. cbn in *.
+          now rewrite it_S in IHi''.
+        * edestruct (IHi (tape_move_right tape1) rest (f x)) as (tape2&IHi'&IHi'').
+          eapply H''. cbn in *.
+          unfold step at 2. cbn. rewrite H'. cbn.
+          unfold step at 2 in IHi''. cbn in IHi''. rewrite E1 in IHi''. cbn in IHi''.
+          eexists tape2. split; auto. cbn in *.
+          now rewrite it_S in IHi''.
+      + exfalso. destruct i; cbn in *.
+        * eapply tape_local_current_cons in H''. enough (None = Some false) by discriminate. rewrite <- E1. auto.
+        * eapply tape_local_current_cons in H''. enough (None = Some  true) by discriminate. rewrite <- E1. auto.
+  Qed.
+
+  Lemma Fin_Seq_terminates_in :
+    Fin_Seq_TM ↓ (fun tapes1 i => exists k, tape_encodes_locally _ (tapes1[@Fin.F1]) k /\ i = S k).
+  Proof.
+    hnf. intros tapes ? (k&(rest&H1)&->). destruct_tapes. cbn in *. hnf in *.
+    destruct (@Fin_Seq_terminates_in_Strong h rest k start) as (?&?&?); eauto.
+  Qed.
+
+  Definition Fin_Seq_R_p : Rel (tapes bool_fin 1) (option X * tapes bool_fin 1) :=
+    ignoreParam (@skip_locally_R 1 Fin.F1 nat _) ∩
+                (fun tps1 '(ox, _) => forall n, tape_encodes_locally _ (tps1[@Fin.F1]) n -> ox = Some (it f n start)).
+
+  Lemma Fin_Seq_WRealise : Fin_Seq ⊫ Fin_Seq_R_p.
+    hnf. intros. destruct_tapes. cbn in *. split; hnf in *.
+    - intros x rest HEnc.
+      pose proof @Fin_Seq_terminates_in_Strong h rest _ start HEnc as (tape2&H1&H2).
+      unfold loopM in *. pose proof (loop_functional H H2) as ->. cbn. auto.
+    - intros x (rest&HEnc).
+      pose proof @Fin_Seq_terminates_in_Strong h rest _ start HEnc as (tape2&H1&H2).
+      unfold loopM in *. pose proof (loop_functional H H2) as ->. cbn. auto.
+  Qed.
+
+End Fin_Seq_TM.
+
+
+
+(* TODO: Instanciate the above TM witch FinStep and Fin.F1 *)
 Section FinMod.
 
   Definition modstep (n : nat) : nat -> nat :=
@@ -44,7 +143,7 @@ Section FinMod.
     intros x. destruct (Fin.to_nat x).
     apply (Fin.of_nat_lt (modstep_le l)).
   Defined.
-  
+
   Lemma fin_next_correct_S (n : nat) (x : Fin.t (S n)) :
     proj1_sig (Fin.to_nat x) < n ->
     proj1_sig (Fin.to_nat (FinStep x)) = S (proj1_sig (Fin.to_nat x)).
@@ -73,129 +172,11 @@ Section FinMod.
     Unset Printing Coercions.
   Qed.
 
-  Definition Fin_plus_mod (n : nat) : nat -> Fin.t (S n) -> Fin.t (S n) := it (@FinStep n).
-
-  Compute Fin_plus_mod (n := 2) 0 (Fin.F1).
-  Compute Fin_plus_mod (n := 2) 1 (Fin.F1).
-  Compute Fin_plus_mod (n := 2) 2 (Fin.F1).
-  Compute Fin_plus_mod (n := 2) 3 (Fin.F1).
-
-  (* Property of it *)
-  Lemma FinStep_S (n : nat) i x :
-    FinStep (Fin_plus_mod (n := n) i x) = Fin_plus_mod (n := n) i (FinStep x).
-  Proof.
-    unfold Fin_plus_mod. induction i; cbn; eauto. now rewrite IHi.
-  Qed.
-    
-  (* Todo: Show that Fin.t is a ring with Fin_plus_mod *)
+  (*
+  Compute it (FinStep (n := 2)) 0 (Fin.F1).
+  Compute it (FinStep (n := 2)) 1 (Fin.F1).
+  Compute it (FinStep (n := 2)) 2 (Fin.F1).
+  Compute it (FinStep (n := 2)) 3 (Fin.F1).
+  *)
+  
 End FinMod.
-
-
-(* Stupid lemma *)
-Section TM_terminates_in_final_state.
-  Variable sig : finType.
-  Variable n : nat.
-  Variable M : mTM sig n.
-
-  Lemma tm_terminates_in_final_state (c1 : mconfig sig (states M) n) (i : nat) :
-    halt (cstate c1) = true ->
-    exists c2 : mconfig sig (states M) n,
-      loopM i c1 = Some c2.
-  Proof. intros H1. exists c1. unfold loopM. Search loop. apply loop_ge with (k1 := 0). omega. cbn. now rewrite H1. Qed.
-    
-End TM_terminates_in_final_state.
-
-
-(* Decode Fin.t *)
-Section Modulo_TM.
-
-  Variable n : nat.
-
-  Print Mk_Mono_TM.
-
-  (* (inl Fin.F1) is the initial state,
-   * (inl _) are the internal states,
-   * (inr _) are the final states, that stand for the corresponding decoding. *)
-  Definition modulo_states := FinType (EqType (Fin.t (S n) + Fin.t (S n)))%type.
-
-  Definition modulo_TM_trans_mono :
-    modulo_states -> option bool_fin -> modulo_states * (option bool_fin * move).
-  Proof.
-    intros q. destruct q as [x | y] eqn:E.
-    - (* inl x *)
-      intros [ [ | ] | ].
-      + (* Some true *)
-        apply (inl (FinStep x), (None, R)). (* increase *)
-      + (* Some false *)
-        apply (inr x, (None, R)). (* terminate *)
-      + (* None *)
-       apply (inl x, (None, N)). (* unexpected end of tape -> diverge *)
-    - (* inr y *)
-      intros _. apply (inr y, (None, N)). (* terminal state *)
-  Defined.
-
-  Definition modulo_fin : modulo_states -> bool.
-  Proof.
-    destruct 1 as [ _ | _ ]; [apply false | apply true].
-  Defined.
-  
-  Definition Modulo_TM : mTM bool_fin 0.
-  Proof.
-    apply Mk_Mono_TM with (states := modulo_states).
-    - apply modulo_TM_trans_mono.
-    - apply (inl (@Fin.F1 n)).
-    - apply modulo_fin.
-  Defined.
-
-  Definition Modulo : { M : mTM bool_fin 0 & states M -> option (Fin.t (S n)) }.
-  Proof.
-    exists Modulo_TM. intros [ _ | x ]; [apply None | apply (Some x)].
-  Defined.
-
-
-  Lemma Modulo_Fin_terminates_in_Strong :
-    forall (tape1 : tape bool_fin) (rest : list bool_fin) (i : nat)
-      (x : Fin.t (S n)),
-      tape_local tape1 = encode i ++ rest ->
-      exists tape2, tape_local tape2 = rest /\
-               loopM (M := Modulo_TM) (S i) (mk_mconfig (inl x) [|tape1|]) =
-               Some (mk_mconfig (inr (Fin_plus_mod i x)) [|tape2|]).
-  Proof.
-    intros tape1 rest i. revert tape1 rest. induction i; intros; cbn in *.
-    - unfold modulo_fin. cbn.
-      unfold step at 1. cbn.
-      replace (current tape1) with (Some false); [ | erewrite tape_local_current_cons; now eauto]. cbn.
-      unfold step at 1. cbn.
-      replace (current tape1) with (Some false); [ | erewrite tape_local_current_cons; now eauto]. cbn.
-      exists (tape_move_right tape1). split; auto. erewrite tape_local_move_right; eauto.
-    - assert (current tape1 = Some true) as H' by (erewrite tape_local_current_cons; eauto).
-      assert (tape_local (tape_move_right tape1) = encode_list encode_unit (repeat tt i) ++ rest)
-        as H'' by (erewrite tape_local_move_right; eauto).
-      unfold step at 1. cbn. rewrite !H'.
-      unfold modulo_fin at 1. cbn.
-      unfold step at 2. unfold step at 2. cbn. rewrite !H'. cbn.
-      unfold step at 2. cbn. rewrite !H'. cbn.
-
-      (* current (tape_move_right tape1) must not be None *)
-      destruct (current (tape_move_right tape1)) eqn:E1.
-      + destruct e eqn:E2; cbn in *.
-        * edestruct (IHi (tape_move_right tape1) rest ((FinStep x))) as (tape2&IHi'&IHi'').
-          eapply H''. cbn in *.
-          unfold step at 2. cbn. rewrite H'. cbn.
-          unfold step at 2 in IHi''. cbn in IHi''. rewrite E1 in IHi''. cbn in IHi''.
-          eexists tape2. split; auto. cbn in *.
-          replace (Fin_plus_mod i (FinStep x)) with (FinStep (Fin_plus_mod i x)) in IHi''. apply IHi''.
-          apply FinStep_S.
-        * edestruct (IHi (tape_move_right tape1) rest (FinStep x)) as (tape2&IHi'&IHi'').
-          eapply H''. cbn in *.
-          unfold step at 2. cbn. rewrite H'. cbn.
-          unfold step at 2 in IHi''. cbn in IHi''. rewrite E1 in IHi''. cbn in IHi''.
-          eexists tape2. split; auto. cbn in *.
-          replace (Fin_plus_mod i (FinStep x)) with (FinStep (Fin_plus_mod i x)) in IHi''. apply IHi''.
-          apply FinStep_S.
-      + exfalso. destruct i; cbn in *.
-        * eapply tape_local_current_cons in H''. enough (None = Some false) by discriminate. rewrite <- E1. auto.
-        * eapply tape_local_current_cons in H''. enough (None = Some  true) by discriminate. rewrite <- E1. auto.
-  Qed.
-  
-End Modulo_TM.
